fixing Reduce.

theories/RTac/Reduce.v
@@ -1,11 +1,14 @@
+Require Import Morphisms.
 Require Import ExtLib.Core.RelDec.
 Require Import ExtLib.Structures.Monad.
+Require Import ExtLib.Data.HList.
 Require Import ExtLib.Tactics.
 Require Import MirrorCore.ExprDAs.
 Require Import MirrorCore.InstantiateI.
 Require Import MirrorCore.RTac.Core.
 
 Require Import MirrorCore.Util.Forwardy.
+Require Import MirrorCore.Util.Nat.
 
 Set Implicit Arguments.
 Set Strict Implicit.
@@ -42,6 +45,171 @@ Section parameterized.
         GConj_ (instantiateGoal f a) (instantiateGoal f b)
     end.
 
+  Definition GExs_nil_check (tes : list (typ * option expr))
+             (g : Goal typ expr) : Goal typ expr :=
+    match tes with
+      | nil => g
+      | _ :: _ => GExs tes g
+    end.
+
+  Theorem GExs_nil_check_respects tus tvs tes
+  : (EqGoal (tus ++ map fst tes) tvs ==> EqGoal tus tvs)%signature
+         (@GExs typ expr tes) (GExs_nil_check tes).
+  Proof.
+    red. intros; subst.
+    unfold EqGoal in *. simpl.
+    destruct tes.
+    { simpl in *.
+      rewrite goalD_conv with (pfu := HList.app_nil_r_trans tus)
+                              (pfv := eq_refl).
+      autorewrite with eq_rw.
+      inversion H; constructor.
+      clear - H2; do 5 red; intros; equivs.
+      rewrite and_comm.
+      rewrite Data.Prop.And_True_iff.
+      rewrite HList.hlist_app_nil_r.
+      autorewrite with eq_rw.
+      eapply H2; reflexivity. }
+    { simpl in *.
+      inversion H; try constructor.
+      match goal with
+        | |- _ _ match ?X with _ => _ end
+                 match ?Y with _ => _ end =>
+          change Y with X ; destruct X
+      end; constructor.
+      clear - H2; do 5 red; intros; equivs.
+      Lemma exists_iff : forall (T : Type) (P Q : T -> Prop),
+                           (forall x, P x <-> Q x) ->
+                           ((exists x, P x) <-> (exists x, Q x)).
+      Proof.
+        clear. intros. setoid_rewrite H. reflexivity.
+      Qed.
+      eapply exists_iff. intros.
+      eapply Quant._exists_iff. intros.
+      eapply and_iff. reflexivity.
+      intros. eapply H2; reflexivity. }
+  Qed.
+
+  Definition GExs_consolidate (tes : list (typ * option expr))
+             (g : Goal typ expr) : Goal typ expr :=
+    match g with
+      | GExs tes' g' => GExs (tes ++ tes') g'
+      | _ => GExs_nil_check tes g
+    end.
+
+  Lemma Proper_GExs
+  : forall tus tvs tes,
+      Proper (EqGoal (tus ++ map fst tes) tvs ==> EqGoal tus tvs)%signature
+             (GExs tes).
+  Proof.
+    clear; intros.
+    red. red. unfold EqGoal.
+    simpl. inversion 1; try constructor.
+    destruct (goal_substD tus tvs (map fst tes) (map snd tes)); constructor.
+    do 5 red; intros; equivs.
+    eapply Quant._exists_iff. intros.
+    eapply and_iff. reflexivity.
+    intros. eapply H2; reflexivity.
+  Qed.
+
+  Lemma goal_substD_app
+  : forall ts' es' tvs ts tus es s1 s2,
+      goal_substD tus tvs ts es = Some s1 ->
+      goal_substD (tus ++ ts) tvs ts' es' = Some s2 ->
+      exists s3,
+        goal_substD tus tvs (ts ++ ts') (es ++ es') = Some s3 /\
+        forall us us' us'' vs,
+          (s1 (hlist_app us us') vs /\
+           s2 (hlist_app (hlist_app us us') us'') vs)
+          <-> s3 (hlist_app us (hlist_app us' us'')) vs.
+  Proof.
+    induction ts; simpl; intros.
+    { forward. subst. inv_all; subst. simpl in *.
+      admit. }
+    { forward. subst. destruct o; forward; inv_all; subst.
+      { specialize (IHts (tus ++ a :: nil) l).
+  Admitted.
+
+  Theorem GExs_consolidate_respects tus tvs tes
+  : forall x y,
+      (EqGoal (tus ++ map fst tes) tvs)%signature x y ->
+      goal_substD tus tvs (map fst tes) (map snd tes) <> None ->
+      (EqGoal tus tvs)%signature
+         (@GExs typ expr tes x) (GExs_consolidate tes y).
+  Proof.
+    intros; subst.
+    destruct y;
+    try solve [ simpl; eapply GExs_nil_check_respects; eauto ].
+    etransitivity.
+    eapply Proper_GExs. eassumption.
+    inversion H; try congruence.
+    { unfold EqGoal. simpl.
+      forward.
+      repeat rewrite map_app.
+      rewrite goalD_conv with (pfu := HList.app_ass_trans tus (map fst tes) (map fst l))
+                                (pfv := eq_refl).
+      autorewrite with eq_rw.
+      destruct (goalD ((tus ++ map fst tes) ++ map fst l) tvs y); try constructor.
+      { forward. admit. } }
+    { unfold EqGoal. simpl.
+      repeat rewrite map_app.
+      rewrite goalD_conv with (pfu := HList.app_ass_trans tus (map fst tes) (map fst l))
+                                (pfv := eq_refl).
+      autorewrite with eq_rw.
+      forward.
+      destruct (goal_substD_app _ _ _ _ _ H0 H4) as [ ? [ ? ? ] ].
+      rewrite H7. constructor.
+      admit. }
+  Qed.
+
+(*
+  5 (None :: Some e :: None :: nil)
+  5 -> 5
+  6 -> e
+  7 -> 6
+*)
+
+  Variable UVar : nat -> expr.
+  Fixpoint adjust' (ls : list (option expr)) (d u : nat) : option expr :=
+    match ls , u with
+      | nil , _ => Some (UVar (d + u))
+      | None :: ls' , 0 => Some (UVar d)
+      | Some e :: ls' , 0 =>
+        Some e (** TODO: I might need to instantiate this **)
+      | None :: ls' , S u => adjust' ls' (S d) u
+      | Some e :: ls' , S u => adjust' ls' d u
+    end.
+
+  Definition adjust (ls : list (option expr)) (nus u : nat) : option expr :=
+    match lt_rem u nus with
+      | None => None
+      | Some r => adjust' ls nus r
+    end.
+
+  Fixpoint GExs_reduce' (tes : list (typ * option expr)) (g : Goal typ expr)
+           (nus : nat) (acc : list (typ * option expr)) (k : list (option expr))
+  : Goal typ expr * nat :=
+    match tes with
+      | nil =>
+        let g' := instantiateGoal (adjust (List.rev k) nus) g in
+        (GExs_nil_check (List.rev acc) g', nus)
+      | te :: tes' =>
+        match te with
+          | (_,None) =>
+            GExs_reduce' tes' g (pred nus) (te :: acc) (None :: k)
+          | (_,Some e) =>
+            (** TODO: I probably want to do my instantiation here! **)
+            GExs_reduce' tes' g (pred nus) acc (Some e :: k)
+        end
+    end.
+
+  Definition GExs_reduce (tes : list (typ * option expr)) (g : Goal typ expr)
+             (nus : nat) : Goal typ expr * nat :=
+    GExs_reduce' tes g nus nil nil.
+
+  Eval cbv beta iota zeta delta - [ lt_rem instantiateGoal ] in
+      fun t g e => GExs_reduce' ((t,None) :: (t,Some e) :: (t,Some e) :: nil) g 0 nil nil.
+
   Fixpoint toGoal (ctx ctx' : Ctx typ expr)
            (cs : ctx_subst subst (Ctx_append ctx ctx')) (g : Goal typ expr)
            (su : nat)
@@ -61,14 +229,10 @@ Section parameterized.
       | CHyp ctx' h => fun cs =>
         @toGoal ctx ctx'  (fromHyp cs) (GHyp h g) 0 un vn
       | CExs ctx' ts => fun cs =>
-        match un with
-          | 0 => (** STUCK **)
-            Fail
-          | S un' =>
-            let '(s,cs') := fromExs cs in
-            let nes := forgets un' ts s in
-            @toGoal ctx ctx' cs' (GExs (List.combine ts nes) g) (S su) un' vn
-        end
+        let '(s,cs') := fromExs cs in
+        let nes := forgets (un - length ts) ts s in
+        let '(g',nus') := GExs_reduce (List.combine ts nes) g un in
+        @toGoal ctx ctx' cs' g' (S su) nus' vn
     end cs.
 
   (** This assumes that the goal is a [GSolved] **)
@@ -95,8 +259,13 @@ Section parameterized.
             Fail
           | S un' =>
             let '(s,cs') := fromExs cs in
-            let nes := forgets un' ts s in
-            @toGoal ctx ctx' cs' (GExs (List.combine ts nes) GSolved) (S su) un' vn
+            let nes := forgets (un - length ts) ts s in
+            let '(g',nus') := GExs_reduce (List.combine ts nes) GSolved un in
+            match g' with
+              | GSolved => @solveGoal ctx ctx' cs' (S su) un' vn
+              | g' => @toGoal ctx ctx' cs' g' (S su) (S nus') vn
+            end
+(*            @toGoal ctx ctx' cs' (GExs (List.combine ts nes) GSolved) (S su) un' vn *)
         end
     end cs.
 
